BoogieExprTranslator/CommonBpl.bpl
@@ -1,20 +1,308 @@
 ﻿// Common code for P semantics
+//Deep copy is guarenteed because, every time we mutate a value, we create a new PrtRef for it.
 
 // Sequences
-procedure {:inline} WriteSeq(seq: PrtRef, index: int, value: PrtRef)  returns (nseq: PrtRef);
+procedure WriteSeq(seq: PrtRef, index: int, value: PrtRef)  returns (nseq: PrtRef)
+{
+    var oldStore: [int]PrtRef;
+    var newStore: [int]PrtRef;
+    int i;
+    int size;
+
+    assert SeqIndexInBounds(seq, index);
+        
+    i := 0;
+    size := PrtFieldSeqSize(seq);
+    oldStore := PrtFieldSeqStore(seq);
+    while(i < size)
+    {
+        if(i == index)
+        {
+            newStore[index] := value;
+        }
+        else
+        {
+            newStore[i] := oldStore[i];
+        }
+        i := i + 1;
+    }
+
+    call nseq := AllocatePrtRef();
+    assume PrtFieldSeqSize(nseq) == size;
+    assume PrtFieldSeqStore(nseq) == newStore;
+    return;
+}
+
+//COME BACK
 procedure {:inline} InsertSeq(seq: PrtRef, index: int, value: PrtRef)  returns (nseq: PrtRef);
-procedure {:inline} RemoveSeq(seq: PrtRef, index: int)  returns (nseq: PrtRef);
+/*{
+
+    var store: [int]PrtRef;
+    var size: int;
+    size := PrtFieldSeqSize(seq);
+    
+    //ToDo: Come Back
+    assert (size  ==  index); //or le?
+    
+    store := PrtFieldSeqStore(seq);
+    store[index] := value;
+
+    call nseq := AllocatePrtRef();
+    assume PrtFieldSeqSize(nseq) == size + 1;
+    assume PrtFieldSeqStore(nseq) == store;
+}
+*/
+
+procedure {:inline} RemoveSeq(seq: PrtRef, index: int)  returns (nseq: PrtRef)
+{
+    var oldStore: [int]PrtRef;
+    var newStore: [int]PrtRef;
+    var size: int;
+    var i: int;
+    
+    size := PrtFieldSeqSize(seq);
+    i := 0;
+    oldStore := PrtFieldSeqStore(seq);
+
+    assert SeqIndexInBounds(seq, index);
+
+    while(i < index)
+    {
+        newStore[i] := oldStore[i];
+        i := i + 1;
+    }
+    while(i < (size - 1))
+    {
+        newStore[i] := oldStore[i + 1];
+        i := i + 1;
+    }
+
+    call nseq := AllocatePrtRef();
+    assume PrtFieldSeqSize(nseq) == size - 1;
+    assume PrtFieldSeqStore(nseq) == newStore;
+    return;
+}
 
 
 // Maps
-procedure {:inline} MapContainsKey(map: PrtRef, key: PrtRef) returns (v: bool);
-procedure {:inline} ReadMap(map: PrtRef, key: PrtRef) returns (value: PrtRef);
-procedure {:inline} MapGetKeys(map: PrtRef) returns (seq: PrtRef);
-procedure {:inline} MapGetValues(map: PrtRef) returns (seq: PrtRef);
+procedure MapContainsKey(map: PrtRef, key: PrtRef) returns (v: bool)
+{
+    var size: int;
+    var i: int;
+    var keys: [int]PrtRef;
 
-procedure {:inline} WriteMap(map: PrtRef, key: PrtRef, value: PrtRef)  returns (nmap: PrtRef);
-procedure {:inline} InsertMap(map: PrtRef, key: PrtRef, value: PrtRef)  returns (nmap: PrtRef);
-procedure {:inline} RemoveMap(map: PrtRef, key: PrtRef)  returns (nmap: PrtRef);
+    v := false;
+    size := PrtFieldMapSize(map);
+    i := 0;
+    keys := PrtFieldMapKeys(map);
+
+    while(i < size)
+    {
+        if(keys[i] == key)
+        {
+            v := true;
+            return;
+        }
+        i := i + 1;
+    }
+    return;
+}
+
+procedure {:inline} ReadMap(map: PrtRef, key: PrtRef) returns (value: PrtRef)
+{
+    var size: int;
+    var i: int;
+    var keys: [int]PrtRef;
+    var values: [int]PrtRef;
+
+    size := PrtFieldMapSize(map);
+    i := 0;
+    keys := PrtFieldMapKeys(map);
+    values := PrtFieldMapValues(map);
+
+    while(i < size)
+    {
+        if(keys[i] == key)
+        {
+            value := values[i];
+            return;
+        }
+        i := i + 1;
+    }
+
+    assert false;
+    return;
+}
+
+procedure {:inline} MapGetKeys(map: PrtRef) returns (seq: PrtRef)
+{
+    var size: int;
+    var oldStore: [int]PrtRef;
+    var newStore: [int]PrtRef;
+    var i: int;
+
+    store := PrtFieldMapKeys(map);
+    size := PrtFieldMapSize(map);
+    i := 0;
+
+    while(i < size)
+    {
+        newStore[i] := oldStore[i];
+        i := i + 1;
+    }
+
+    call seq := AllocatePrtRef();
+    assume PrtFieldSeqStore(seq) == newStore; 
+    assume PrtFieldSeqSize(seq) == size;
+
+    return;
+}
+procedure {:inline} MapGetValues(map: PrtRef) returns (seq: PrtRef)
+{
+    var size: int;
+    var oldStore: [int]PrtRef;
+    var newStore: [int]PrtRef;
+    var i: int;
+
+    store := PrtFieldMapValues(map);
+    size := PrtFieldMapSize(map);
+    i := 0;
+
+    while(i < size)
+    {
+        newStore[i] := oldStore[i];
+        i := i + 1;
+    }
+
+    call seq := AllocatePrtRef();
+    assume PrtFieldSeqStore(seq) == newStore; 
+    assume PrtFieldSeqSize(seq) == size;
+
+    return;
+}
+
+procedure {:inline} WriteMap(map: PrtRef, key: PrtRef, value: PrtRef)  returns (nmap: PrtRef)
+{
+    var size: int;
+    var i: int;
+    var flag: bool;
+    var oldKeys: [int]PrtRef;
+    var oldValues: [int]PrtRef;
+    var newKeys: [int]PrtRef;
+    var newValues: [int]PrtRef;
+
+    size := PrtFieldMapSize(map);
+    i := 0;
+    oldKeys := PrtFieldMapKeys(map);
+    oldValues := PrtFieldMapValues(map);
+    flag := false;
+
+    while(i < size)
+    {
+        newKeys[i] := oldKeys[i];
+        if(oldKeys[i] == key)
+        {
+            newValues[i] := value;
+            flag := true;
+        }
+        else
+        {
+            newValues[i] := oldValues[i];
+        }
+        i := i + 1;
+    }
+
+    assert flag;
+
+    call nmap := AllocatePrtRef();
+    assume PrtFieldMapSize(nmap) == size;
+    assume PrtFieldMapKeys(nmap) == newKeys;
+    assume PrtFieldMapValues(nmap) == newValues;
+
+    return;
+}
+
+procedure {:inline} InsertMap(map: PrtRef, key: PrtRef, value: PrtRef)  returns (nmap: PrtRef)
+{
+    var size: int;
+    var i: int;
+    var oldKeys: [int]PrtRef;
+    var oldValues: [int]PrtRef;
+    var newKeys: [int]PrtRef;
+    var newValues: [int]PrtRef;
+
+    size := PrtFieldMapSize(map);
+    i := 0;
+    oldKeys := PrtFieldMapKeys(map);
+    oldValues := PrtFieldMapValues(map);
+    
+    while(i < size)
+    {
+        newKeys[i] := oldKeys[i];
+        newValues[i] := oldValues[i];
+        if(oldKeys[i] == key)
+        {
+            assert false;
+        }
+        i := i + 1;
+    }
+    
+    newKeys[i] := key;
+    newValues[i] := value;
+
+    call nmap := AllocatePrtRef();
+    assume PrtFieldMapSize(nmap) == size + 1;
+    assume PrtFieldMapKeys(nmap) == newKeys;
+    assume PrtFieldMapValues(nmap) == newValues;
+
+    return;
+}
+
+procedure RemoveMap(map: PrtRef, key: PrtRef)  returns (nmap: PrtRef)
+{
+    var size: int;
+    var i: int;
+    var flag: bool;
+    var oldKeys: [int]PrtRef;
+    var oldValues: [int]PrtRef;
+    var newKeys: [int]PrtRef;
+    var newValues: [int]PrtRef;
+
+    size := PrtFieldMapSize(map);
+    assert (size > 0);
+    i := 0;
+    oldKeys := PrtFieldMapKeys(map);
+    oldValues := PrtFieldMapValues(map);
+    flag := false;
+
+    while(i < size && oldkeys[i] != key)
+    {
+        newKeys[i] := oldKeys[i];
+        newValues[i] := oldValues[i];
+        if(oldKeys[i] == key)
+        {
+            flag := true;
+            newKeys[i] := oldKeys[size - 1];
+            newValues[i] := oldValues[size - 1];
+        }
+        i := i + 1;
+    }
+    assert flag;
+
+    while(i < (size - 1))
+    {
+        newKeys[i] := oldKeys[i + 1];
+        newValues[i] := oldValues[i + 1];
+        i := i + 1;
+    }
+
+    call nmap := AllocatePrtRef();
+    assume PrtFieldMapSize(nmap) == size - 1;
+    assume PrtFieldMapKeys(nmap) == newKeys;
+    assume PrtFieldMapValues(nmap) == newValues;
+
+    return;
+}
 
 
 //The global counter for machines.
